src/L1To2Refinement/Definitions.v
@@ -1,5 +1,4 @@
-Require Import Primitives Layer1 Layer2 BlockAllocatorDefinitions.
-Require Import SimulationLayer.
+Require Import Primitives Simulation Layer1 Layer2 BlockAllocator.
 Close Scope pred_scope.
 Import ListNotations.
 
@@ -9,8 +8,8 @@ Fixpoint compile {T} (p2: Layer2.prog T) : Layer1.prog T :=
     | Write a v => write a v
     | Alloc v => alloc v
     | Free a => free a
-    | Ret v => Layer1Definitions.Ret v
-    | Bind px py => Layer1Definitions.Bind (compile px) (fun x => compile (py x))
+    | Ret v => Layer1.Ret v
+    | Bind px py => Layer1.Bind (compile px) (fun x => compile (py x))
     end.
 
 (* October 12: I need oracle_ok in here because specifications of block allocator requires it as a precondition *)
@@ -18,9 +17,9 @@ Fixpoint oracle_refines_to T (d1: State layer1_lts) (p: Layer2.prog T)  (o1: Ora
   oracle_ok (compile p) o1 d1 /\
     match p with
     | Alloc v =>
-      if (in_dec Layer1Definitions.token_dec Layer1Definitions.Crash o1) then
+      if (in_dec Layer1.token_dec Layer1.Crash o1) then
         forall d1',
-          Layer1Definitions.exec o1 d1 (compile p) (Crashed d1') ->
+          Layer1.exec o1 d1 (compile p) (Crashed d1') ->
           let sv := Disk.read d1 0 in
           let sv' := Disk.read d1' 0 in
           match sv, sv' with
@@ -49,34 +48,34 @@ Fixpoint oracle_refines_to T (d1: State layer1_lts) (p: Layer2.prog T)  (o1: Ora
     | @Bind T1 T2 p1 p2 =>
       exists o1' o1'',
       o1 = o1'++o1'' /\
-     ((exists d1', Layer1Definitions.exec o1 d1 (compile p1) (Crashed d1') /\
+     ((exists d1', Layer1.exec o1 d1 (compile p1) (Crashed d1') /\
          oracle_refines_to T1 d1 p1 o1 o2 /\ o1'' = []) \/
       (exists d1' r ret,
-          Layer1Definitions.exec o1' d1 (compile p1) (Finished d1' r) /\
-          Layer1Definitions.exec o1'' d1' (compile (p2 r)) ret /\
+          Layer1.exec o1' d1 (compile p1) (Finished d1' r) /\
+          Layer1.exec o1'' d1' (compile (p2 r)) ret /\
          exists o2' o2'',
          oracle_refines_to T1 d1 p1 o1' o2' /\
          oracle_refines_to T2 d1' (p2 r) o1'' o2'' /\
          o2 = o2' ++ o2''))
     | Read _ =>
-      if (in_dec Layer1Definitions.token_dec Layer1Definitions.Crash o1) then
+      if (in_dec Layer1.token_dec Layer1.Crash o1) then
         o2 = [Crash1]
       else
         o2 = [Cont]
     | Ret _ =>
-      if (in_dec Layer1Definitions.token_dec Layer1Definitions.Crash o1) then
+      if (in_dec Layer1.token_dec Layer1.Crash o1) then
         o2 = [Crash1]
       else
         o2 = [Cont]
     | Free _ =>
-      if (in_dec Layer1Definitions.token_dec Layer1Definitions.Crash o1) then
+      if (in_dec Layer1.token_dec Layer1.Crash o1) then
         o2 = [Crash1]
       else
         o2 = [Cont]
     | Write a _ =>
-      if (in_dec Layer1Definitions.token_dec Layer1Definitions.Crash o1) then
+      if (in_dec Layer1.token_dec Layer1.Crash o1) then
          forall d1',
-          Layer1Definitions.exec o1 d1 (compile p) (Crashed d1') ->
+          Layer1.exec o1 d1 (compile p) (Crashed d1') ->
           let sv := d1 a in
           let sv' := d1' a in
           match sv, sv' with
