src/BlockAllocator.v
@@ -1,3 +1,0 @@
-Require Export BlockAllocatorDefinitions.
-Require Export BlockAllocatorFacts.
-Require Export BlockAllocatorSpecs.
