src/BlockAllocator/Definitions.v
@@ -1,4 +1,4 @@
-Require Import Primitives Omega Disk ListUtils.
+Require Import Primitives Layer1 Omega.
 Close Scope pred_scope.
 
 Axiom block_size: nat.
