src/Layer1.v
@@ -1,5 +1,0 @@
-Require Export Layer1Definitions Layer1Facts.
-Notation "'Layer1.state'" := Layer1Definitions.state.
-Notation "'Layer1.oracle'" := Layer1Definitions.oracle.
-Notation "'Layer1.prog'" := Layer1Definitions.prog.
-Notation "'Layer1.exec'" := Layer1Definitions.exec.
