src/Layer1/HoareLogic.v
@@ -1,0 +1,381 @@
+Require Import Primitives Simulation Layer1.Definitions ProgAuto.
+
+Set Implicit Arguments.
+
+
+(** ** Hoare logic *)
+Definition precond := oracle -> @pred addr addr_dec (set value).
+Definition postcond {T: Type} := T -> @pred addr addr_dec (set value).
+Definition crashcond := @pred addr addr_dec (set value).
+
+
+Definition hoare_triple {T: Type} (pre: precond) (p: prog T) (post: @postcond T) (crash: crashcond):=
+  forall o d,
+    pre o d ->
+    (exists ret,
+        exec o d p ret /\
+        ((exists d' r,
+             ret = Finished d' r
+             /\ post r d') \/
+         (exists d',
+             ret = Crashed d' /\ crash d')))%type.
+
+
+  
+Notation
+  "<< o >> pre p << r >> post crash" :=
+  (forall F, hoare_triple
+          (fun o d => (F * pre * [[ oracle_ok p o d ]]) d)%pred
+          p%pred
+          (fun r => F * post)%pred
+          (F * crash)%pred)
+    (at level 10, o at next level, pre at next level, p at next level, r at next level, post at next level, crash at next level,
+     format "'[v' '[  ' '<<' o '>>' '//' '[' pre ']' '//' '[' p ']' ']' '//' '[  ' '<<' r '>>' '//' '[' post ']' '//' '[' crash ']' ']' ']'").
+
+(*
+Notation
+  "{{ e1 }} << o >> pre p << r >> post crash" :=
+   (exists e1, (forall F, hoare_triple
+          (fun o => F * pre)%pred
+          p
+          (fun r => F * post)%pred
+          (F * crash)%pred))
+    (at level 10, o at next level, pre at next level, p at next level, r at next level, post at next level, crash at next level,
+     format "'[v' '{{' e1 '}}' '//' '[  ' '<<' o '>>' '//' pre '//' p ']' '//' '[  ' '<<' r '>>' '//' post '//' crash ']' ']'").
+*)
+
+Theorem hoare_triple_strengthen_pre:
+  forall T (p: prog T) (pre pre': precond) post crash,
+  hoare_triple pre p post crash ->
+  (forall o, pre' o =p=>  pre o) ->
+  hoare_triple pre' p post crash.
+Proof.
+  unfold hoare_triple; intros;
+    edestruct H; intros; eauto.
+  eapply H0; eauto.
+Qed.
+
+(*
+Theorem hoare_triple_weaken_post_weak:
+  forall T (p: prog T) pre (post post': postcond) crash,
+  hoare_triple pre p post crash ->
+  (forall  o d r,
+      pre o d ->
+      post r =p=>
+      post' r) ->
+  hoare_triple pre p post' crash.
+Proof.
+  unfold hoare_triple; intros;
+    edestruct H; intros; eauto.
+  cleanup; split_ors; cleanup.
+  eexists; split; eauto.  
+  left; repeat eexists; eauto.
+  eapply H0; eauto.
+  eexists; split; eauto.
+Qed.
+
+
+Theorem hoare_triple_weaken_post_strong:
+  forall T (p: prog T) pre (post post': postcond) crash,
+  hoare_triple pre p post crash ->
+  (forall o d (r: T),
+      post o d r =p=>
+      post' o d r) ->
+  hoare_triple pre p post' crash.
+Proof.
+  intros; eapply hoare_triple_weaken_post_weak; eauto.
+Qed.
+
+Theorem hoare_triple_weaken_crash_weak:
+  forall T (p: prog T) pre post (crash crash': crashcond),
+  hoare_triple pre p post crash ->
+  (forall o d,
+      pre o d ->
+      crash o d =p=>
+      crash' o d) ->
+  hoare_triple pre p post crash'.
+Proof.
+  unfold  hoare_triple; intros;
+    edestruct H; intros; eauto.
+  cleanup; split_ors; cleanup.
+  eexists; split; eauto.
+  eexists; split; eauto.  
+  right; repeat eexists; eauto.
+  eapply H0; eauto. 
+Qed.
+
+
+Theorem hoare_triple_weaken_crash_strong:
+  forall T (p: prog T) pre post (crash crash': crashcond),
+  hoare_triple pre p post crash ->
+  (forall o d, crash o d =p=> crash' o d) ->
+  hoare_triple pre p post crash'.
+Proof.
+  intros; eapply hoare_triple_weaken_crash_weak; eauto.
+Qed.
+
+
+Theorem hoare_triple_pimpl :
+    forall T1 T2 (p1: prog T1) (p2: T1 -> prog T2) (pre: precond) pre1 post1 pre2 post2 crash1 crash2,
+      hoare_triple pre1 p1 post1 crash1 ->
+      (forall o d,
+          pre o d ->
+          exists o1 o2,
+            o = o1++o2 /\
+            (o2 = [] \/ ~In Crash o1) /\
+            pre1 o1 d) ->
+      (forall o1 d,
+         pre1 o1 d ->
+         (forall o2 r, post1 r =p=> pre2 o2)) ->
+      (forall o1 d r,
+         pre1 o1 d ->
+         (forall o2, post1 r =p=> pre2 o2) ->
+          hoare_triple pre2 (p2 r) post2 crash2) ->
+    (forall o d,
+      pre1 o d ->
+      crash1 =p=> crash2) ->
+    hoare_triple pre (Bind p1 p2) post2 crash2.
+Proof.
+  unfold hoare_triple; intros.
+  edestruct H0; eauto; cleanup.
+  edestruct H; eauto; cleanup.
+  specialize H1 with (1:=H7).
+  specialize H3 with (1:=H7).
+  split_ors.
+  - (* p1 Finished *)    
+    edestruct H2; eauto.
+    eapply H1; eauto.
+    cleanup.
+    split_ors; cleanup.
+    + (* p2 Finished *)
+      clear H8.
+      eexists; split; eauto.
+      left; do 2 eexists; intuition eauto.
+      eapply H4; eauto.
+      eapply H1; eauto.
+    + (* p2 Crashed *)
+      clear H8.
+      eexists. intuition eauto.
+      right; eexists; intuition eauto.
+      eapply H5; eauto.
+      eapply H1; eauto.
+  - (* p1 Crashed *)
+    split_ors; cleanup.
+    eexists. intuition eauto.
+    cleanup; rewrite app_nil_r;
+      econstructor; eauto.
+    cleanup; rewrite app_nil_r; eauto.
+    apply exec_crash_in in H7; intuition.   
+Qed.
+*)
+
+Theorem hoare_triple_equivalence :
+  forall T (p p': prog T) pre post crash,
+    hoare_triple pre p post crash ->
+    prog_equiv p p' ->
+    hoare_triple pre p' post crash.
+Proof.
+  unfold hoare_triple; intros.
+  edestruct H; eauto; cleanup.
+  match goal with
+  | [ H: _ ~= _ |- _ ] =>
+    edestruct H; eauto
+  end.
+Qed.
+
+
+Ltac monad_simpl_one :=
+  match goal with
+  | [ |- hoare_triple _ (Bind (Bind _ _) _) _ _ ] =>
+    eapply hoare_triple_equivalence;
+    [ | apply bind_assoc ]
+  end.
+
+Ltac monad_simpl := repeat monad_simpl_one.
+
+Theorem bind_ok:
+  forall T T' (p1: prog T) (p2: T -> prog T') pre1 post1 crash1 pre2 post2 crash2 crash3,
+  << o >>
+   pre1
+   p1
+  << r >>
+   (post1 r)
+   crash1 ->
+  (forall F d r,
+      (F * pre1)%pred d ->
+      post1 r =p=> pre2) ->
+  (forall F d,
+      (F * pre1)%pred d ->
+      crash1 =p=> crash3) ->
+  (forall F d1 d2 r1,
+      (F * pre1)%pred d1 ->
+      (F * post1 r1)%pred d2 ->
+      (F * pre2)%pred d2 ->
+      crash2 =p=> crash3) ->
+  (forall F d d' r,
+      (F * pre1)%pred d ->
+      (F * post1 r)%pred d' ->
+      << o >>
+         pre2
+         (p2 r)
+       << r >>
+       (post2 r)
+       crash2) ->
+  << o >>
+     pre1
+     (Bind p1 p2)
+  << r >>
+     (post2 r)
+     crash3.
+Proof.
+  unfold hoare_triple; intros.
+  simpl in *; destruct_lifts; cleanup.
+  edestruct H; eauto.
+  pred_apply' H4; cancel; eauto.
+  
+  cleanup.
+  split_ors; cleanup.
+  - specialize H7 with (1:=H5).
+    edestruct H3; eauto.
+    pred_apply' H10; norm.
+    cancel.
+    erewrite H0; eauto; cancel.
+    intuition eauto.
+
+    cleanup.
+    split_ors; cleanup;
+    eexists; split; intuition eauto.
+    
+    right; eexists; intuition eauto.
+    pred_apply; cancel; eauto.
+    eapply H2; eauto.
+    erewrite <- H0; eauto.
+  - specialize H8 with (1:=H5); cleanup.
+    rewrite app_nil_r.
+    eexists; split; intuition eauto.
+    right; eexists; intuition eauto.
+    pred_apply; cancel.
+    eauto.
+Qed.
+
+
+Theorem crash_weaken:
+  forall T (p: prog T) pre post crash1 crash2,
+  << o >>
+   pre
+   p
+  << r >>
+   (post r)
+   crash1 ->
+  (crash1 =p=> crash2) ->
+  << o >>
+     pre
+     p
+  << r >>
+     (post r)
+     crash2.
+Proof.
+  unfold hoare_triple; intros.
+  edestruct H; eauto.
+  cleanup.
+  split_ors; cleanup;
+    eexists; intuition eauto.
+  right; eexists; intuition eauto.
+  pred_apply; cancel; eauto.
+Qed.
+
+
+Theorem post_weaken:
+  forall T (p: prog T) pre post1 post2 crash,
+  << o >>
+   pre
+   p
+  << r >>
+   (post1 r)
+   crash  ->
+  (forall r, post1 r =p=> post2 r) ->
+  << o >>
+     pre
+     p
+  << r >>
+     (post2 r)
+     crash.
+Proof.
+  unfold hoare_triple; intros.
+  edestruct H; eauto.
+  cleanup.
+  split_ors; cleanup;
+    eexists; intuition eauto.
+  left; do 2 eexists; intuition eauto.
+  pred_apply; cancel; eauto.
+Qed.
+
+Theorem pre_strengthen:
+  forall T (p: prog T) pre1 pre2 post crash,
+  << o >>
+   pre1
+   p
+  << r >>
+   (post r)
+   crash ->
+  (pre2 =p=> pre1) ->
+  << o >>
+     pre2
+     p
+  << r >>
+     (post r)
+     crash.
+Proof.
+  unfold hoare_triple; intros.
+  edestruct H; eauto.
+  pred_apply; cancel; eauto.
+Qed.
+
+
+Theorem add_frame:
+  forall T (p: prog T) pre post crash F,
+  << o >>
+   pre
+   p
+  << r >>
+   (post r)
+   crash  ->
+  << o >>
+     (F * pre)
+     p
+  << r >>
+     (F * post r)
+     (F * crash).
+Proof.
+  unfold hoare_triple; intros.
+  edestruct H; eauto.
+  pred_apply' H0; cancel; eauto.
+  cleanup; split_ors; cleanup;
+    eexists; intuition eauto.
+  left; do 2 eexists; intuition eauto.
+  pred_apply; cancel; eauto.
+  right; eexists; intuition eauto.
+  pred_apply; cancel; eauto.
+Qed.
+
+Theorem extract_exists:
+  forall T V (p: prog T) pre post crash,
+    (forall (v:V),
+  << o >>
+   (pre v)
+   p
+  << r >>
+   (post r)
+   crash) ->
+  << o >>
+     (exists v, pre v)
+     p
+  << r >>
+     (post r)
+     crash.
+Proof.
+  unfold hoare_triple; intros.
+  destruct_lifts.
+  eapply H; eauto.
+  pred_apply' H0; cancel; eauto.
+Qed.
