src/Layer1/Layer1.v
@@ -1,0 +1,11 @@
+Require Export HoareLogic Layer1.Specs ProgAuto.
+Require Export Layer1.Definitions Layer1.Facts.
+Notation "'Layer1.state'" := Layer1.Definitions.state.
+Notation "'Layer1.oracle'" := Layer1.Definitions.oracle.
+Notation "'Layer1.prog'" := Layer1.Definitions.prog.
+Notation "'Layer1.exec'" := Layer1.Definitions.exec.
+Notation "'Layer1.token_dec'" := Layer1.Definitions.token_dec.
+Notation "'Layer1.Ret'" := Layer1.Definitions.Ret.
+Notation "'Layer1.Bind'" := Layer1.Definitions.Bind.
+Notation "'Layer1.Cont'" := Layer1.Definitions.Cont.
+Notation "'Layer1.Crash'" := Layer1.Definitions.Crash.
