src/Layer2.v
@@ -1,5 +1,0 @@
-Require Export Layer2Definitions Layer2Facts.
-Notation "'Layer2.state'" := Layer2Definitions.state.
-Notation "'Layer2.oracle'" := Layer2Definitions.oracle.
-Notation "'Layer2.prog'" := Layer2Definitions.prog.
-Notation "'Layer2.exec'" := Layer2Definitions.exec.
