src/Layer2/Layer2.v
@@ -1,0 +1,5 @@
+Require Export Layer2.Definitions Layer2.Facts.
+Notation "'Layer2.state'" := Layer2.Definitions.state.
+Notation "'Layer2.oracle'" := Layer2.Definitions.oracle.
+Notation "'Layer2.prog'" := Layer2.Definitions.prog.
+Notation "'Layer2.exec'" := Layer2.Definitions.exec.
