src/Primitives.v
@@ -1,4 +1,0 @@
-Require Export List BaseTypes Memx Predx SepAuto.
-Require Export Disk Simulation Layer1 ProgAuto HoareL1.
-Require Export OpSpec CommonAutomation.
-Export ListNotations.
